\documentclass[12pt,fleqn]{article}
\usepackage[russian]{babel}
\usepackage[utf8]{inputenc}
\usepackage{amsmath,amssymb, amsthm}
\setlength{\parindent}{0pt}
\begin{document}
Solve the equation
$$- \frac{\log{\left (x \right )}}{\log{\left (10 \right )}} + \frac{\log{\left (\frac{x + 8}{x - 1} \right )}}{\log{\left (10 \right )}} = 0$$
Rewrite the equation as
$$\frac{1}{\log{\left (10 \right )}} \left(- \log{\left (x \right )} + \log{\left (\frac{x + 8}{x - 1} \right )}\right) = 0$$
Solve the equation
$$- \log{\left (x \right )} + \log{\left (\frac{x + 8}{x - 1} \right )} = 0$$
Rewrite the equation as
$$\log{\left (\frac{x + 8}{x - 1} \right )} = \log{\left (x \right )}$$
Therefore we get
$$\frac{x + 8}{x - 1} = x$$
Solve the equation
$$- x + \frac{x + 8}{x - 1} = 0$$
Rewrite the equation as
$$\frac{1}{x - 1} \left(- x \left(x - 1\right) + x + 8\right) = 0$$
Solve the equation
$$- x \left(x - 1\right) + x + 8 = 0$$
Rewrite the equation as
$$- x^{2} + 2 x + 8 = 0$$
This equation is quadratic
The discriminant is
$$D = 36$$
Use the formulas
$$x = \frac{-2 + \sqrt{36}}{-1 \cdot 2}$$
$$x = \frac{- 6 - 2}{-1 \cdot 2}$$
Therefore the roots of this quadratic equation are
$$x = -2$$
$$x = 4$$
\end{document}
