\documentclass[12pt,fleqn]{article}
\usepackage[russian]{babel}
\usepackage[utf8]{inputenc}
\usepackage{amsmath,amssymb, amsthm}
\setlength{\parindent}{0pt}
\begin{document}
Solve the equation
$$- \frac{\log{\left (- x \right )}}{\log{\left (5 \right )}} + \frac{\log{\left (x^{2} - 12 \right )}}{\log{\left (5 \right )}} = 0$$
Rewrite the equation as
$$\frac{1}{\log{\left (5 \right )}} \left(- \log{\left (- x \right )} + \log{\left (x^{2} - 12 \right )}\right) = 0$$
Solve the equation
$$- \log{\left (- x \right )} + \log{\left (x^{2} - 12 \right )} = 0$$
Rewrite the equation as
$$\log{\left (x^{2} - 12 \right )} = \log{\left (- x \right )}$$
Therefore we get
$$x^{2} - 12 = - x$$
Solve the equation
$$x^{2} + x - 12 = 0$$
This equation is quadratic
The discriminant is
$$D = 49$$
Use the formulas
$$x = \frac{1}{2} \left(-1 + \sqrt{49}\right)$$
$$x = \frac{1}{2} \left(- 7 - 1\right)$$
Therefore the roots of this quadratic equation are
$$x = 3$$
$$x = -4$$
\end{document}
